16: proof Relax_Edges pt.1

Matei.dfy
@@ -1,81 +1,7 @@
-datatype Weight = W(val: int)
 datatype Node = V(id: int)
-
-datatype Edge = Edge(source: Node, destination: Node, weight: Weight)
-datatype Graph = Graph(nodes: set<Node>, edges: set<Edge>)
-
-function edge_weight(e: Edge): int
-{
-  match e
-  case Edge(from_where, to_where, W(w)) => w
-}
-
-function from_where(e: Edge): Node
-{
-  match e
-  case Edge(from_where, to_where, W(w)) => from_where
-}
-
-function to_where(e: Edge): Node
-{
-  match e
-  case Edge(from_where, to_where, W(w)) => to_where
-}
-
-function nodes_in_graph(g: Graph): set<Node>
-{
-  match g
-  case Graph(v, e) => v
-}
-
-function edges_in_graph(g: Graph): set<Edge>
-{
-  match g
-  case Graph(v, e) => e
-}
-
-predicate isValid(graph: Graph)
-{
-  forall e :: e in graph.edges ==> e.source in graph.nodes && e.destination in graph.nodes
-}
-
-
-method Main(){
-  var node1 := V(1);
-  var node2 := V(2);
-  var node3 := V(3);
-
-  var edge1 := Edge(node1, node2, W(2));
-  var edge2 := Edge(node2,node3, W(4));
-
-  var graph1 := Graph({node1,node2,node3}, {edge1,edge2});
-}
-
-
-predicate EmptySet<T(==)>() { {} is set<T> }
-
-method check_if_set_empty(s: set<int>) returns (IsEmpty:bool)
-{
-  IsEmpty := s == {};
-}
-
+datatype New_Weight = W_new(val: MyInt)
+datatype New_Edge = Edge_new(source: Node, destination: Node, weight: New_Weight)
 datatype MyInt = Valid(n: int) | MinValue
-
-method testMinValue(x: MyInt) returns (isMin: bool)
-{
-  isMin := match x {
-    case MinValue => true
-    case Valid(_) => false
-  };
-}
-
-function MyIntToInt(x: MyInt): int
-  requires x != MinValue
-{
-  match x {
-    case Valid(n) => n
-  }
-}
 
 function MyIntAdd(x: MyInt, y: MyInt): MyInt
 {
@@ -101,13 +27,16 @@ function MyIntLessThan(x: MyInt, y: MyInt): bool
   }
 }
 
-datatype New_Weight = W_new(val: MyInt)
-datatype New_Edge = Edge_new(source: Node, destination: Node, weight: New_Weight)
-
 method Relax_Edges(source: Node, predecessor: array<int>, edges: array<New_Edge>, distance: array<MyInt>)
   modifies distance, predecessor
+  requires distance.Length > 0 && edges.Length > 0 && predecessor.Length > 0
+  requires predecessor.Length == distance.Length
+  requires forall edge: New_Edge :: edge in seq(edges) ==>
+                                      0 <= edge.source.id < distance.Length && 0 <= edge.destination.id < distance.Length
+
 {
-  if distance.Length == 0 || edges.Length == 0 || predecessor.Length == 0 {
+  if distance.Length == 0 || edges.Length == 0 || predecessor.Length == 0
+  {
     return;
   }
 
@@ -126,8 +55,10 @@ method Relax_Edges(source: Node, predecessor: array<int>, edges: array<New_Edge>
       var v := edge.destination.id;
       var w := edge.weight.val;
 
-      if 0 <= u < distance.Length && 0 <= v < distance.Length && 0 <= v < predecessor.Length {
-        if distance[u] != MinValue && MyIntLessThan(MyIntAdd(distance[u], w), distance[v]) {
+      if 0 <= u < distance.Length && 0 <= v < distance.Length && 0 <= v < predecessor.Length
+      {
+        if distance[u] != MinValue && MyIntLessThan(MyIntAdd(distance[u], w), distance[v])
+        {
           distance[v] := MyIntAdd(distance[u], w);
           predecessor[v] := u;
         }
@@ -136,21 +67,5 @@ method Relax_Edges(source: Node, predecessor: array<int>, edges: array<New_Edge>
     }
     i := i + 1;
   }
-}
-
-method hasNegativeCycle(graph: Graph) returns (hasNegative: bool)
-{
-  var nodess := graph.nodes;
-  var edgess := graph.edges;
-
-  if nodess == {} {
-    hasNegative := false;
-    return;
-  }
-  else{
-    hasNegative := true;
-    return;
-  }
 
 }
-
